feat: iota verified

lean/Shars/Verification/Iota.lean
@@ -11,287 +11,56 @@ import Shars.Verification.Constants
 import Shars.Verification.Utils
 import Shars.Verification.Auxiliary
 
-set_option maxHeartbeats 1000000
-
 open Aeneas hiding Std.Array
 open Std.alloc.vec
 
-theorem algos.IOTA_RC_POINTS.spec
-: ∀ t < 255, IOTA_RC_POINTS.val[t]! = Spec.Keccak.ι.rc t
+attribute [-simp] List.getElem!_eq_getElem?_getD
+attribute [ext (iff := false)] List.ext_getElem!
+
+theorem algos.IOTA_RC.spec
+: ∀ iᵣ < 24, IOTA_RC.val[iᵣ]!.toBits = (Spec.Keccak.ι.RC (l := 6) iᵣ).toList
 := by native_decide
 
-attribute [scalar_tac_simps] Nat.mod_mod Fin.ofNat'
-
-@[progress]
-theorem algos.iota_rc_point.spec(t: Std.Usize)
-: ∃ output,
-  iota_rc_point t = .ok output ∧
-  output = Spec.Keccak.ι.rc t.val
+theorem List.ext_toBits{bs1 bs2: List (Bool)}
+  (len_bs1: bs1.length = Spec.b 6)
+  (len_bs2: bs2.length = Spec.b 6)
+  (point_eq: ∀ (x y: Fin 5)(z: Fin (Spec.w 6)), bs1[Spec.Keccak.StateArray.encodeIndex x y z]! = bs2[Spec.Keccak.StateArray.encodeIndex x y z]!)
+: bs1 = bs2
 := by
-  simp [iota_rc_point]
-  progress*
-  simp [*, IOTA_RC_POINTS.spec (t.val % 255) (by scalar_tac), Spec.Keccak.ι.rc_mod_eq_rc]
-
-def algos.iota_rc_init_loop.ref(ir: Nat)(rc: BitVec (Spec.w 6))(j: Nat) :=
-  if j <= 6
-  then
-    let i := 7 * ir
-    let i1 := j + i
-    let b := Spec.Keccak.ι.rc i1
-    let i2 := 1 <<< j
-    let i3 := i2 - 1
-    let rc1 := rc.set i3 b
-    let j1 := j + 1
-    iota_rc_init_loop.ref ir rc1 j1
-  else rc
-termination_by 7 - j
-
-theorem algos.iota_rc_init_loop.ref_spec(ir : Std.Usize) (input : Aeneas.Std.Array Bool 64#usize)(j: Std.Usize)
-: ir.val < 24
-→ j.val ≤ 6 + 1
-→ ∃ output,
-  iota_rc_init_loop ir input j = .ok output ∧
-  output.val.toBitVec.cast (by simp [Spec.w]) = algos.iota_rc_init_loop.ref ir.val (input.val.toBitVec.cast (by simp [Spec.w])) j.val
-:= by
-  intro ir_lt j_loop_bound
-  rw [iota_rc_init_loop, iota_rc_init_loop.ref]
-  split
-  case isTrue j_lt =>
-    let* ⟨ i, i_post ⟩ ← Std.Usize.mul_spec
-    let* ⟨ i1, i1_post ⟩ ← Std.Usize.add_spec
-    let* ⟨ b, b_post ⟩ ← iota_rc_point.spec
-    simp [i1_post, i_post] at b_post
-    let* ⟨ i2, i2_post_1, i2_post_2 ⟩ ← Std.Usize.one_ShiftLeft_spec
-    · have:= Std.UScalarTy.Usize_numBits_le
-      scalar_tac
-    let* ⟨ i3, i3_post ⟩ ← Std.Usize.sub_spec
-    have i3_idx: i3.val < input.length := by
-      simp [*]
-      calc  2 ^ ↑j - 1
-          _ < 2 ^ ↑j := Nat.pred_lt (Nat.ne_of_gt (Nat.two_pow_pos j.val))
-          _ ≤ 2 ^ 6 := Nat.pow_le_pow_right Nat.two_pos (by simpa using j_lt)
-    let* ⟨ rc1, rc1_post ⟩ ← Std.Array.update_spec
-    let* ⟨ j1, j1_post ⟩ ← Std.Usize.add_spec
-    let* ⟨ res, res_post ⟩ ← ref_spec
-    -- END PROGRESS
-    rw [res_post, ←BitVec.cast_set (i_idx := ?first)]
-    case first =>
-      simp [Nat.shiftLeft_eq, NatCast.natCast, Fin.ofNat']
-      rw [Nat.mod_eq_of_lt] <;> simpa [*] using i3_idx
-    rw [rc1_post, List.toBitVec, Std.Array.set, BitVec.ofBoolListLE_set (i_idx := by simpa using i3_idx)]
-    simp
-    simp_ifs
-    congr 3
-    simp [*]
-    rw [Nat.shiftLeft_eq, Nat.one_mul, Nat.mod_eq_of_lt]
-    simpa [*] using i3_idx
-  case isFalse => simp [‹j.val = 7›']
-termination_by 7 - j.val
-decreasing_by scalar_decr_tac
-
-theorem algos.iota_rc_init_loop.ref.foldWhile_spec(iᵣ: Nat)(input: BitVec (Spec.w 6))(j: Nat)
-: iota_rc_init_loop.ref iᵣ input j = SRRange.foldWhile
-    (i    := j)
-    (max  := 6 + 1)
-    (step := 1) (hStep := Nat.one_pos)
-    (init := input)
-    (f    := fun input j => input.set (↑(1 <<< j - 1)) (Spec.Keccak.ι.rc (j + 7 * iᵣ)))
-:= by
-  rw [ref, SRRange.foldWhile]
-  if h: j < 7 then
-    simp only
-    simp [h, ‹j ≤ 6›']
-    rw [algos.iota_rc_init_loop.ref.foldWhile_spec]
-  else simp [h, ‹¬ (j ≤ 6)›']
-
-def Spec.Keccak.ι.RC.loop (iᵣ: Nat)(init: BitVec (w 6))(start: Nat): BitVec (w 6) := Id.run do
-  let mut RC := init
-  for j in List.finRange (6 + 1) |>.drop start do
-    have j_valid_idx := calc  2 ^ ↑j - 1
-        _ < 2 ^ ↑j := Nat.pred_lt (Nat.ne_of_gt (Nat.two_pow_pos j.val))
-        _ ≤ 2 ^ 6 := Nat.pow_le_pow_right Nat.two_pos <| Fin.is_le j
-    RC := RC.set ⟨2^j.val - 1, j_valid_idx⟩ (ι.rc (↑j + 7*iᵣ))
-  return RC
-
-theorem Spec.Keccak.ι.RC.loop_refinement(iᵣ: Nat)
-: RC.loop iᵣ (0#(w 6)) 0 = RC iᵣ
-:= by simp [loop, RC]; congr
-
-theorem Spec.Keccak.ι.RC.loop.foldl_spec(iᵣ: Nat)(init: BitVec (w 6))(start: Nat)
-: RC.loop iᵣ init start =
-    List.foldl (fun RC j => RC.set! (2^j - 1) (ι.rc (j + 7*iᵣ))) init (List.range (6 + 1) |>.drop start)
-:= by
-  simp [RC.loop]
-  rw [
-    ←List.val_finRange_eq_range 7,
-    ←List.map_drop,
-    ←List.foldl_of_foldl_map (f := Fin.val)
-  ]
-  ext RC j : 2
-  rw [BitVec.set!_eq_set]
-
-theorem Aeneas.SRRange.foldWhile_eq_foldWhile'{α : Type u}
-(i max step : Nat) (hStep : 0 < step) (f : α → Nat → α) (init : α)(start: Nat)
-: (cond: start ≤ i ∧ (i - start) % step = 0)
-→ foldWhile max step hStep f i init = SRRange.foldWhile' {
-    start := start
-    stop  := max
-    step  := step
-    step_pos := hStep
-  } (fun acc e _ => f acc e) i init (hi := by simp [cond])
-:= by
-  intro ⟨start_le, start_modeq_i⟩
-  unfold foldWhile foldWhile'
-  simp
-  split
-  · rw [Aeneas.SRRange.foldWhile_eq_foldWhile']
-    constructor
-    · omega
-    · rw [Nat.add_comm i, Nat.add_sub_assoc (start_le)]
-      simp [start_modeq_i]
-  · rfl
-termination_by max - i
-
-def algos.iota_rc_init_loop.foldWhile.spec(iᵣ: Nat)(init: BitVec (Spec.w 6))(start: Nat)
-: SRRange.foldWhile
-    (i    := start)
-    (max  := 6 + 1)
-    (step := 1) (hStep := Nat.one_pos)
-    (init := init)
-    (f    := fun input j => BitVec.set (1 <<< j - 1).cast (Spec.Keccak.ι.rc (j + 7 * iᵣ)) input)
-= Spec.Keccak.ι.RC.loop iᵣ init start
-:= by
-  rw [Spec.Keccak.ι.RC.loop.foldl_spec, List.drop_range, SRRange.foldl_range'_eq_foldWhile (hStep := Nat.one_pos)]
-  simp
-  if start_idx: start < 7 then
-    rw [‹start  + (7 - start) = 7›']
-    rw [SRRange.foldWhile_eq_foldWhile' (start:=start) (cond := by simp)]
-    rw [SRRange.foldWhile_eq_foldWhile' (start:=start) (cond := by simp)]
-    congr
-    ext input j j_idx : 3
-    rw [←BitVec.set!_eq_set]
-    congr 2
-    simp
-    simp only [Nat.shiftLeft_eq, Nat.one_mul]
-    simp [Membership.mem] at j_idx
-    have j_valid_idx := calc  2 ^ j - 1
-        _ < 2 ^ j := Nat.pred_lt (Nat.ne_of_gt (Nat.two_pow_pos j))
-        _ ≤ 2 ^ 6 := Nat.pow_le_pow_right Nat.two_pos (by scalar_tac)
-    rw [Nat.mod_eq_of_lt]; simpa using j_valid_idx
-  else
-    rw [SRRange.foldWhile_id (h := start_idx), SRRange.foldWhile_id (h := by simpa using start_idx)]
-
-@[progress]
-theorem algos.iota_rc_init_loop.spec(ir : Std.Usize) (input : Aeneas.Std.Array Bool 64#usize)(i: Std.Usize)
-: ir.val < 24
-→ i.val ≤ 6 + 1
-→ ∃ output,
-  algos.iota_rc_init_loop ir input i = .ok output ∧
-  output.val.toBitVec.cast (by simp [Spec.w]) = Spec.Keccak.ι.RC.loop ir.val (input.val.toBitVec.cast (by simp [Spec.w])) i.val
-:= by
-  intro ir_lt i_loop_bound
-  let* ⟨ output, output_post⟩ ← iota_rc_init_loop.ref_spec
-  rw [
-    output_post,
-    algos.iota_rc_init_loop.ref.foldWhile_spec,
-    algos.iota_rc_init_loop.foldWhile.spec,
-  ]
-
-set_option maxRecDepth 1000000 in
-@[progress]
-theorem algos.iota_rc_init.spec(ir: Std.Usize)
-: ir.val < 24
-→ ∃ output,
-  algos.iota_rc_init ir (Std.Array.repeat 64#usize false) = .ok output ∧
-  output.val.toBitVec.cast (by simp [Spec.w]) = (Spec.Keccak.ι.RC ir.val : BitVec (Spec.w 6))
-:= by
-  intro ir_lt
-  simp [iota_rc_init]
-  let* ⟨output , output_post⟩ ← iota_rc_init_loop.spec
-  rw [output_post, ←Spec.Keccak.ι.RC.loop_refinement]
-  rfl
-
-@[progress]
-theorem algos.iota_a_loop.spec(res : StateArray) (a : StateArray) (rc : Aeneas.Std.Array Bool 64#usize)(z: Std.Usize)
-: ∃ output,
-  algos.iota_a_loop res a rc z = .ok output ∧
-  ∀ (x y: Fin 5)(z': Fin (Spec.w 6)),
-  output.toSpec.get x y z' =
-    if x = 0 ∧ y = 0 ∧ z.val ≤ z'.val then
-      a.toSpec.get 0 0 z' ^^ rc.val.toBitVec[z'.val]!
-    else
-      res.toSpec.get x y z'
-:= by
-  rw [algos.iota_a_loop]
-  split
-  case isTrue =>
-    let* ⟨ b, b_post ⟩ ← StateArray.index.spec
-    let* ⟨ b1, b1_post ⟩ ← Std.Array.index_usize_spec
-    let* ⟨ b2, b2_post ⟩ ← binxor.spec
-    simp [b_post, b1_post] at b2_post
-    let* ⟨ old_res, set_res, old_res_post, set_res_post ⟩ ← StateArray.index_mut.spec
-    let* ⟨ z1, z1_post ⟩ ← Std.Usize.add_spec
-    let* ⟨ rest, rest_post ⟩ ← spec
-    simp [*] at rest_post
-    intro x y z'
-    rw [rest_post]
-    split_all
-    · simp [Spec.Keccak.StateArray.get_set]
-    · scalar_tac
-    · simp [Spec.Keccak.StateArray.get_set]
-      have zz' := ‹z.val = z'.val›'
-      simp only [Fin.isValue, zz', Fin.cast_val_eq_self, and_true]--, ite_eq_left_iff, not_and]
-      simp_ifs
-    · rw [Spec.Keccak.StateArray.get_set]
-      have: ¬ (x = 0 ∧ y = 0 ∧ z' = z.val.cast) := by
-        -- TODO: Could we modify `scalar_tac` so that it handles this case?
-        -- The issue is with `Fin` inequalities being hiden behind `And`, `Or` or `Not`.
-        -- It would be nice to have `scalar_tac` transform these using the lemmas
-        --  · Fin.val_fin_le
-        --  · Fin.val_inj
-        -- I was thinking of using a `simproc`, but I don't think these work with
-        -- implications, since they're supposed to do rewritings.
-        -- Perhaps I could have it
-        rename_i h1 h2
-        simp [not_and_or, -not_and] at h1 h2 ⊢
-        rcases h1 with (h1 | h1 | h1) <;> try simp [h1]
-        rcases h2 with (h1 | h1 | h1) <;> try simp [h1]
-        right;right
-        intro aux
-        replace aux := Fin.val_eq_of_eq aux
-        simp [Nat.mod_eq_of_lt, ‹z.val < Spec.w 6›'] at aux
-        scalar_tac
-      simp_ifs
-  case isFalse z_oob =>
-    simp at z_oob ⊢
-    intro x y z'
-    simp_ifs
-termination_by (Spec.w 6 + 1) - z.val
-decreasing_by scalar_decr_tac
+  apply List.ext_getElem
+  · simp [len_bs1, len_bs2]
+  intro idx idx_lt _
+  simp [len_bs1] at idx_lt
+  have ⟨x, y, z, encode_xyz⟩ := IR.decode_surjective idx idx_lt
+  simp [←encode_xyz, ←getElem!_pos, List.getElem!_encodeIndex_toBits]
+  apply point_eq
 
 @[progress]
 theorem algos.iota.spec(ir: Std.Usize)(input: StateArray)
 : ir.val < 24
 → ∃ output,
   iota ir input = .ok output ∧
-  output.toSpec = Spec.Keccak.ι (iᵣ:= ir.val) input.toSpec
+  output.toBits = (Spec.Keccak.ι (iᵣ:= ir.val) input.toSpec).toBits
 := by
   intro ir_lt
-  simp [iota, iota_a, ClonealgosStateArray.clone]
-  let* ⟨rc, rc_post⟩ ← iota_rc_init.spec
-  let* ⟨res, res_post⟩ ← iota_a_loop.spec
-  ext x y z
-  simp only [Spec.Keccak.ι, Spec.Keccak.StateArray.get_ofFn, res_post]
-  split
-  case isTrue h =>
-    simp only [Fin.isValue, h, id_eq, Id.run, Fin.getElem_fin, Id.pure_eq, Spec.Keccak.StateArray.get_ofFn, Bool.bne_right_inj]
-    replace rc_post := BitVec.cast_left _ rc_post
-    rw [rc_post, ←getElem_eq_getElem! (h := by scalar_tac)]
-    simp
-  case isFalse h =>
-    simp
-    split
-    · simp [*] at *
-      simp [*] at *
-    rename_i h; simp at h; obtain ⟨rfl, rfl, rfl⟩ := h
-    rfl
+  rw [iota]
+  simp only [Std.toResult, Std.bind_tc_ok, StateArray.toSpec]
+  progress*
+  simp [*, Std.Array.toBits, Spec.Keccak.ι]
+  apply List.ext_toBits
+  · simp +decide [List.length_toBits]
+  · simp
+  intro x y z
+  rw [Fin.getElem!_fin, IR.encodeIndex_spec, List.getElem!_encodeIndex_toBits (z_lt := z.isLt)]
+  rw [Spec.Keccak.StateArray.getElem!_toBits_encodeIndex, Spec.Keccak.StateArray.get_ofFn]
+  if cond: x = 0 ∧ y = 0 then
+    simp +decide [cond, List.length_toBits, List.get_toStateArray, List.getElem!_encodeIndex_toBits, Std.UScalar.getElem!_xor_toBits]
+    rw [IOTA_RC.spec ir ir_lt]
+    simp [←getElem!_pos]
+  else
+    simp only [not_and_or] at cond
+    obtain h | h := cond
+    all_goals (
+      simp [h]
+      simp +decide [cond, List.length_toBits, List.get_toStateArray, List.getElem!_encodeIndex_toBits]
+    )
