lean/Shars/Verification/Constants.lean
@@ -1,10 +1,8 @@
 import Shars.Definitions.Algos
 
-@[simp, scalar_tac_simps] theorem algos.L.spec: L =    6#usize := by native_decide
-@[simp, scalar_tac_simps] theorem algos.W.spec': W =   64#usize := by native_decide
-@[simp, scalar_tac_simps] theorem algos.B.spec: B = 1600#usize := by native_decide
-
 attribute [local simp] Aeneas.Std.eval_global
 
-@[simp, scalar_tac_simps] theorem algos.SHA3_SUFFIX.spec: SHA3_SUFFIX = ⟨[false, true], by simp⟩ := by simp [SHA3_SUFFIX, SHA3_SUFFIX_body, Aeneas.Std.Array.make]
-@[simp, scalar_tac_simps] theorem algos.SHAKE_SUFFIX.spec: SHAKE_SUFFIX = ⟨[true, true, true, true], by simp⟩ := by simp [SHAKE_SUFFIX, SHAKE_SUFFIX_body, Aeneas.Std.Array.repeat]
+@[simp, scalar_tac_simps] theorem algos.W.spec': W =   64#usize := by simp [W, W_body]
+
+@[simp, scalar_tac_simps] theorem  algos.SHA3_EXTRA.spec: SHA3_EXTRA  = ⟨0b00000110, by decide⟩ := by simp +decide [SHA3_EXTRA, SHA3_EXTRA_body]
+@[simp, scalar_tac_simps] theorem algos.SHAKE_EXTRA.spec: SHAKE_EXTRA = ⟨0b00011111, by decide⟩ := by simp +decide [SHAKE_EXTRA, SHAKE_EXTRA_body]
